feat: simulation proofs in Set and call to top-level functions

CoqOfRust/proofs/M.v
@@ -57,50 +57,50 @@ Definition IsTraitMethod
   List.assoc instance method_name = Some (InstanceField.Method method).
 
 Module Run.
-  Reserved Notation "{{ env , env_to_value , state | e ⇓ result | state' }}".
+  Reserved Notation "{{ env , env_to_value , state | e ⇓ to_value | P_state }}".
 
-  Inductive t `{State.Trait} {Env : Set} (env : Env) (env_to_value : Env -> Value.t)
-      (* Be aware of the order of parameters: the result and final state are at
-         the beginning. This is due to the way polymorphic types for inductive
-         work in Coq, and the fact that the result is always the same as we are
-         in continuation passing style. *)
-      (result : Value.t + Exception.t) (state' : State) :
-      M -> State -> Prop :=
-  | Pure :
-    {{ env, env_to_value, state' | LowM.Pure result ⇓ result | state' }}
+  Inductive t `{State.Trait} {Env A : Set} (env : Env) (env_to_value : Env -> Value.t)
+      (state : State)
+      (to_value : A -> Value.t + Exception.t) (P_state : State -> Prop) :
+      M -> Set :=
+  | Pure
+      (result : A)
+      (result' : Value.t + Exception.t) :
+    result' = to_value result ->
+    P_state state ->
+    {{ env, env_to_value, state | LowM.Pure result' ⇓ to_value | P_state }}
   | CallPrimitiveStateAllocImmediate
-      (state : State) (v : Value.t)
+      (v : Value.t)
       (k : Value.t -> M) :
     {{ env, env_to_value, state |
-      k (Value.Pointer (Pointer.Immediate v)) ⇓ result
-    | state' }} ->
+      k (Value.Pointer (Pointer.Immediate v)) ⇓ to_value
+    | P_state }} ->
     {{ env, env_to_value, state |
-      LowM.CallPrimitive (Primitive.StateAlloc v) k ⇓ result
-    | state' }}
+      LowM.CallPrimitive (Primitive.StateAlloc v) k ⇓ to_value
+    | P_state }}
   | CallPrimitiveStateAllocMutable
       (address : Address)
       (value : State.get_Set address)
       (value' : Value.t)
-      (to_value : State.get_Set address -> Value.t)
-      (state : State)
+      (pointer_to_value : State.get_Set address -> Value.t)
+      (state_inter : State)
       (k : Value.t -> M) :
-    let r := Value.Pointer (Pointer.mutable address to_value) in
-    value' = to_value value ->
+    let r := Value.Pointer (Pointer.mutable address pointer_to_value) in
+    value' = pointer_to_value value ->
     State.read address state = None ->
-    State.alloc_write address state value = Some state' ->
-    {{ env, env_to_value, state | k r ⇓ result | state' }} ->
+    State.alloc_write address state value = Some state_inter ->
+    {{ env, env_to_value, state_inter | k r ⇓ to_value | P_state }} ->
     {{ env, env_to_value, state |
-      LowM.CallPrimitive (Primitive.StateAlloc value') k ⇓ result
-    | state' }}
+      LowM.CallPrimitive (Primitive.StateAlloc value') k ⇓ to_value
+    | P_state }}
   | CallPrimitiveStateRead
-      {A : Set} {to_value : A -> Value.t} address path big_to_value projection injection
+      {A : Set} {pointer_to_value : A -> Value.t} address path big_to_value projection injection
       (value : State.get_Set address)
       (sub_value : A)
-      (state : State)
       (k : Value.t -> M) :
     let mutable :=
       Pointer.Mutable.Make
-        (Value := Value.t) (A := A) (to_value := to_value) (Address := Address)
+        (Value := Value.t) (A := A) (to_value := pointer_to_value) (Address := Address)
         (Big_A := State.get_Set address)
         address
         path
@@ -110,84 +110,93 @@ Module Run.
     State.read address state = Some value ->
     projection value = Some sub_value ->
     {{ env, env_to_value, state |
-      k (to_value sub_value) ⇓
-      result
-    | state' }} ->
+      k (pointer_to_value sub_value) ⇓
+      to_value
+    | P_state }} ->
     {{ env, env_to_value, state |
       LowM.CallPrimitive (Primitive.StateRead mutable) k ⇓
-      result
-    | state' }}
+      to_value
+    | P_state }}
   | CallPrimitiveStateWrite
-      {A : Set} {to_value : A -> Value.t} address path big_to_value projection injection
+      {A : Set} {pointer_to_value : A -> Value.t} address path big_to_value projection injection
       (value : A) (value' : Value.t)
       (big_value new_big_value : State.get_Set address)
-      (state state_inter : State)
+      (state_inter : State)
       (k : Value.t -> M) :
     let mutable :=
       Pointer.Mutable.Make
-        (Value := Value.t) (A := A) (to_value := to_value) (Address := Address)
+        (Value := Value.t) (A := A) (to_value := pointer_to_value) (Address := Address)
         (Big_A := State.get_Set address)
         address
         path
         big_to_value
         projection
         injection in
-    value' = to_value value ->
+    value' = pointer_to_value value ->
     State.read address state = Some big_value ->
     injection big_value value = Some new_big_value ->
     State.alloc_write address state new_big_value = Some state_inter ->
-    {{ env, env_to_value, state_inter | k (Value.Tuple []) ⇓ result | state' }} ->
+    {{ env, env_to_value, state_inter | k (Value.Tuple []) ⇓ to_value | P_state }} ->
     {{ env, env_to_value, state |
       LowM.CallPrimitive (Primitive.StateWrite mutable value') k ⇓
-      result
-    | state' }}
-  | CallPrimitiveGetSubPointer {A Sub_A : Set} {to_value : A -> Value.t}
-      (mutable : Pointer.Mutable.t Value.t to_value)
+      to_value
+    | P_state }}
+  | CallPrimitiveGetSubPointer {A Sub_A : Set} {pointer_to_value : A -> Value.t}
+      (mutable : Pointer.Mutable.t Value.t pointer_to_value)
       index sub_projection sub_injection sub_to_value
-      (state : State)
       (k : Value.t -> M) :
     (* Communtativity of the read *)
     (forall (a : A),
       Option.map (sub_projection a) sub_to_value =
-      Value.read_path (to_value a) [index]
+      Value.read_path (pointer_to_value a) [index]
     ) ->
     (* Communtativity of the write *)
     (forall (a : A) (sub_a : Sub_A),
-      Option.map (sub_injection a sub_a) to_value =
-      Value.write_value (to_value a) [index] (sub_to_value sub_a)
+      Option.map (sub_injection a sub_a) pointer_to_value =
+      Value.write_value (pointer_to_value a) [index] (sub_to_value sub_a)
     ) ->
     {{ env, env_to_value, state |
       k (Value.Pointer (Pointer.Mutable (Pointer.Mutable.get_sub
         mutable index sub_projection sub_injection sub_to_value
       ))) ⇓
-      result
-    | state' }} ->
+      to_value
+    | P_state }} ->
     {{ env, env_to_value, state |
       LowM.CallPrimitive (Primitive.GetSubPointer mutable index) k ⇓
-      result
-    | state' }}
+      to_value
+    | P_state }}
   | CallPrimitiveEnvRead
-      (state : State) (k : Value.t -> M) :
-    {{ env, env_to_value, state | k (env_to_value env) ⇓ result | state' }} ->
+      (k : Value.t -> M) :
+    {{ env, env_to_value, state | k (env_to_value env) ⇓ to_value | P_state }} ->
     {{ env, env_to_value, state |
-      LowM.CallPrimitive Primitive.EnvRead k ⇓ result
-    | state' }}
+      LowM.CallPrimitive Primitive.EnvRead k ⇓ to_value
+    | P_state }}
+  | CallPrimitiveGetFunction
+      (name : string) (generic_tys : list Ty.t)
+      (function : list Ty.t -> list Value.t -> M)
+      (k : Value.t -> M) :
+    let closure :=
+      Value.Closure (existS (Value.t, M) (function generic_tys)) in
+    M.IsFunction name function ->
+    {{ env, env_to_value, state | k closure ⇓ to_value | P_state }} ->
+    {{ env, env_to_value, state |
+      LowM.CallPrimitive (Primitive.GetFunction name generic_tys) k ⇓
+      to_value
+    | P_state }}
   | CallPrimitiveGetAssociatedFunction
-      (state : State)
       (ty : Ty.t) (name : string) (generic_tys : list Ty.t)
       (associated_function : list Ty.t -> list Value.t -> M)
       (k : Value.t -> M) :
     let closure :=
       Value.Closure (existS (Value.t, M) (associated_function generic_tys)) in
     M.IsAssociatedFunction ty name associated_function ->
-    {{ env, env_to_value, state | k closure ⇓ result | state' }} ->
+    {{ env, env_to_value, state | k closure ⇓ to_value | P_state }} ->
     {{ env, env_to_value, state |
       LowM.CallPrimitive
         (Primitive.GetAssociatedFunction ty name generic_tys) k ⇓
-        result
-    | state' }}
+        to_value
+    | P_state }}
   | CallPrimitiveGetTraitMethod
-      (state : State)
       (trait_name : string) (self_ty : Ty.t) (trait_tys : list Ty.t)
       (method_name : string) (generic_tys : list Ty.t)
       (method : list Ty.t -> list Value.t -> M)
@@ -195,7 +204,7 @@ Module Run.
     let closure :=
       Value.Closure (existS (Value.t, M) (method generic_tys)) in
     IsTraitMethod trait_name self_ty trait_tys method_name method ->
-    {{ env, env_to_value, state | k closure ⇓ result | state' }} ->
+    {{ env, env_to_value, state | k closure ⇓ to_value | P_state }} ->
     {{ env, env_to_value, state |
       LowM.CallPrimitive
         (Primitive.GetTraitMethod
@@ -205,34 +214,92 @@ Module Run.
           method_name
           generic_tys)
         k ⇓
-        result
-    | state' }}
-  | CallClosure
-      (state state_inter : State)
+        to_value
+    | P_state }}
+  | CallClosure {A_inter : Set}
+      (to_value_inter : A_inter -> Value.t + Exception.t) (P_state_inter : State -> Prop)
       (f : list Value.t -> M) (args : list Value.t)
-      (value : Value.t + Exception.t)
       (k : Value.t + Exception.t -> M) :
     let closure := Value.Closure (existS (Value.t, M) f) in
-    {{ env, env_to_value, state | f args ⇓ value | state_inter }} ->
-    {{ env, env_to_value, state_inter | k value ⇓ result | state' }} ->
-    {{ env, env_to_value, state | LowM.CallClosure closure args k ⇓ result | state' }}
+    {{ env, env_to_value, state | f args ⇓ to_value_inter | P_state_inter }} ->
+    (forall (value_inter : A_inter) (state_inter : State),
+      P_state_inter state_inter ->
+      {{ env, env_to_value, state_inter | k (to_value_inter value_inter) ⇓ to_value | P_state }}
+    ) ->
+    {{ env, env_to_value, state | LowM.CallClosure closure args k ⇓ to_value | P_state }}
 
-  where "{{ env , env_to_value , state | e ⇓ result | state' }}" :=
-    (t env env_to_value result state' e state).
+  where "{{ env , env_to_value , state | e ⇓ to_value | P_state }}" :=
+    (t env env_to_value state to_value P_state e).
 
-  Definition pure (e : M) (result : Value.t + Exception.t) : Prop :=
+  Definition pure {A : Set} (e : M) (to_value : A -> Value.t + Exception.t) : Set :=
     forall
       (State Address : Set) `(State.Trait State Address)
       (Env : Set) (env : Env) (env_to_value : Env -> Value.t)
       (state : State),
-    {{ env, env_to_value, state | e ⇓ result | state }}.
+    {{ env, env_to_value, state |
+      e ⇓ to_value
+    | fun state' => state' = state }}.
 End Run.
+
+Import Run.
+
+Fixpoint evaluate `{State.Trait} {Env A : Set}
+    {env : Env} {env_to_value : Env -> Value.t} {state : State}
+    {e : M} {to_value : A -> Value.t + Exception.t}
+    {P_state : State -> Prop}
+    (run : {{ env, env_to_value, state | e ⇓ to_value | P_state }}) :
+  A * { state : State | P_state state }.
+Proof.
+  destruct run.
+  { split.
+    { exact result. }
+    { eexists.
+      match goal with
+      | H : P_state _ |- _ => exact H
+      end.
+    }
+  }
+  { eapply evaluate.
+    exact run.
+  }
+  { eapply evaluate.
+    exact run.
+  }
+  { eapply evaluate.
+    exact run.
+  }
+  { eapply evaluate.
+    exact run.
+  }
+  { eapply evaluate.
+    exact run.
+  }
+  { eapply evaluate.
+    exact run.
+  }
+  { eapply evaluate.
+    exact run.
+  }
+  { eapply evaluate.
+    exact run.
+  }
+  { eapply evaluate.
+    exact run.
+  }
+  { destruct (evaluate _ _ _ _ _ _ _ _ _ _ _ run) as [value_inter [state_inter H_state_inter]].
+    eapply evaluate.
+    match goal with
+    | H : forall _ _ _, _ |- _ => apply (H value_inter)
+    end.
+    exact H_state_inter.
+  }
+Defined.
 
 Module SubPointer.
   Module Runner.
     Module Valid.
       Inductive t {A Sub_A : Set} `{ToValue A} `{ToValue Sub_A} :
-          SubPointer.Runner.t A Sub_A -> Prop :=
+          SubPointer.Runner.t A Sub_A -> Set :=
       | Intro
           (index : Pointer.Index.t)
           (projection : A -> option Sub_A)
@@ -257,28 +324,29 @@ Module SubPointer.
 
   Import Run.
 
-  Lemma run
-      {A Sub_A : Set} `{ToValue A} `{ToValue Sub_A}
+  Definition run
+      {Result : Set} {A Sub_A : Set} `{ToValue A} `{ToValue Sub_A}
       {runner : SubPointer.Runner.t A Sub_A}
       (H_runner : Runner.Valid.t runner)
       (mutable : Pointer.Mutable.t (A := A) Value.t φ)
-      `{State.Trait} {Env : Set} (env : Env) (env_to_value : Env -> Value.t)
-      (result : Value.t + Exception.t) (state state' : State) (k : Value.t -> M)
+      `{State.Trait} {Env : Set} (env : Env) (env_to_value : Env -> Value.t) (state : State)
+      (to_value : Result -> Value.t + Exception.t) (P_state : State -> Prop)
+      (k : Value.t -> M)
       (index : Pointer.Index.t) :
     index = runner.(SubPointer.Runner.index) ->
     {{ env, env_to_value, state |
       k (Value.Pointer (Pointer.Mutable (SubPointer.get_sub mutable runner))) ⇓
-      result
-    | state' }} ->
+      to_value
+    | P_state }} ->
     {{ env, env_to_value, state |
       LowM.CallPrimitive (Primitive.GetSubPointer mutable index) k ⇓
-      result
-    | state' }}.
+      to_value
+    | P_state }}.
   Proof.
     intros.
     destruct H_runner.
     eapply Run.CallPrimitiveGetSubPointer; sfirstorder.
-  Qed.
+  Defined.
 End SubPointer.
 
 (** Simplify the usual case of read of immediate value. *)
@@ -291,27 +359,26 @@ Qed.
 
 Ltac run_symbolic_state_read :=
   match goal with
-  | |- Run.t _ _ _ _ (LowM.CallPrimitive (Primitive.StateRead (
+  | |- Run.t _ _ _ _ _ (LowM.CallPrimitive (Primitive.StateRead (
       Pointer.Mutable.Make ?address _ _ _ _
-    )) _) _ =>
+    )) _) =>
     let H := fresh "H" in
-    epose proof (H := Run.CallPrimitiveStateRead _ _ _ _ address);
+    epose proof (H := Run.CallPrimitiveStateRead _ _ _ _ _ address);
     eapply H; [reflexivity | reflexivity |];
     clear H
   end.
 
 Ltac run_symbolic_state_write :=
   match goal with
-  | |- Run.t ?env ?env_to_value ?result ?state'
+  | |- Run.t ?env ?env_to_value ?state ?to_value ?P_state
       (LowM.CallPrimitive (Primitive.StateWrite (
         Pointer.Mutable.Make ?address ?path ?big_to_value ?projection ?injection
-      ) ?value') ?k)
-      ?state =>
+      ) ?value') ?k) =>
     let H := fresh "H" in
     epose proof (H :=
       Run.CallPrimitiveStateWrite
-        env env_to_value result state' address path big_to_value projection injection _
-        value' _ _ _ _ k
+        env env_to_value state to_value P_state address path big_to_value projection injection _
+        value' _ _ _ k
     );
     apply H; try reflexivity;
     clear H
@@ -322,7 +389,7 @@ Ltac run_symbolic_one_step :=
   | |- Run.t _ _ _ _ _ _ =>
     (* We do not use [Run.CallClosure] and let the user use existing lemma
        for this kind of case. *)
-    apply Run.Pure ||
+    (eapply Run.Pure; trivial) ||
     apply Run.CallPrimitiveStateAllocImmediate ||
     apply Run.CallPrimitiveEnvRead ||
     run_symbolic_state_read ||
