CoqOfRust/core/simulations/intrinsics.v
@@ -1,0 +1,30 @@
+Require Import CoqOfRust.CoqOfRust.
+Require Import proofs.M.
+Require Import simulations.M.
+
+Require core.intrinsics.
+
+Import Run.
+
+Definition sub_with_overflow_kind (kind : Integer.t) (x y : Z) : Z * bool :=
+  let z := Integer.normalize_wrap kind (x - y) in
+  let has_overflow := orb (z <? Integer.min kind) (Integer.max kind <? z) in
+  (z, has_overflow).
+
+(* TODO: add the other integer cases *)
+Axiom sub_with_overflow_u64_eq :
+  core.intrinsics.intrinsics.sub_with_overflow [Ty.path "u64"] =
+  fun α =>
+    match α with
+    | [ Value.Integer x; Value.Integer y ] => M.pure (φ (sub_with_overflow_kind Integer.U64 x y))
+    | _ => M.impossible
+    end.
+
+Definition run_sub_with_overflow_u64_u64 (self rhs : Z) :
+  Run.pure (core.intrinsics.intrinsics.sub_with_overflow [Ty.path "u64"] [φ self; φ rhs])
+    (fun (v : (Z * bool)) => inl (φ v)).
+Proof.
+  unfold Run.pure; intros.
+  rewrite sub_with_overflow_u64_eq.
+  with_strategy opaque [sub_with_overflow_kind] run_symbolic.
+Defined.
