CoqOfRust/revm/instructions/simulations/arithmetic.v
@@ -1,0 +1,8 @@
+Require Import CoqOfRust.CoqOfRust.
+Require Import CoqOfRust.proofs.M.
+
+Import Run.
+
+(* Definition run_record_cost 
+
+Definition run_add  *)
